finished proof of SCC algorithm

SCCAlg.v
@@ -569,6 +569,9 @@ Qed.
 (** Defining the second DFS pass **)
 Module D2 := (D' O S G F).
 
+(*The second pass uses DFSCustomOrder, not DFSBase (since the order depends on the graph, and Coq's modules
+  do not allow this. The vertices are ordered in reverse order of their finish times from the first pass. We
+  prove that this is a valid Graphordering*)
 Program Instance reverseF (g: G.graph) : D2.G'.GraphOrdering (G.get_transpose g) 
   (fun v1 v2 => (D1.f_time None g v2) <? (D1.f_time None g v1)) := {
   }.
@@ -584,20 +587,14 @@ repeat(rewrite Nat.ltb_lt). assert ((D1.f_time None g y < D1.f_time None g x) \/
 eapply D1.f_times_unique. apply G.transpose_vertices. apply H.
 apply G.transpose_vertices. apply H0. symmetry.  apply H2.
 Defined. 
-(*
-Next Obligation.
-case_eq (Nat.compare (D1.f_time None g x) (D1.f_time None g y)); intro; simpl in *.
-- apply EQ. unfold O.eq. eapply D1.f_times_unique. apply H. apply H0. apply Nat.compare_eq in H1. apply H1.
-- apply GT. simpl. apply nat_compare_Lt_lt in H1. omega.
-- apply LT. simpl. apply nat_compare_Gt_gt in H1. omega.
-Defined.*)
+
 
 Section SecondPass.
   Variable g' : G.graph.
   Definition gt := G.get_transpose g'.
   Definition lt := (fun v1 v2 => D1.f_time None g' v2 <? D1.f_time None g' v1).
-(*Just a test - ok figure this out tomorrow - can either do backtracking with nats (or more likely for now -
-  just pass a function*)
+
+(*When the root of a tree in the forest is discovered, it has the largest finish time of all remaining vertices*)
 Lemma root_largest_finish_time: forall v (s: D2.state gt lt (reverseF g') None),
   D2.time_of_state gt lt (reverseF g') None s = D2.d_time gt lt (reverseF g') None v ->
   F.is_root (D2.dfs_forest gt lt (reverseF g') None) v = true ->
@@ -610,9 +607,7 @@ Proof.
   rewrite Nat.ltb_lt in H3. apply H3. reflexivity. 
 Qed. 
 
-
-(*For any two trees in the DFS forest, if the root of t1 finishes before the root of t2, then there
-  is no edge rom t1 to t2*)
+(*A few helper lemmas*)
 
 Lemma get_tree_in_graph: forall g lt H o v t,
   InA S.Equal t (F.get_trees (D2.dfs_forest g lt H o)) ->
@@ -624,64 +619,6 @@ Proof.
   rewrite H3 in H1. apply F.desc_in_forest in H1. eapply D2.same_vertices. apply H1. auto.
 Qed.
 
-Lemma no_edge_to_later_tree: forall g lt H o v1 v2 r1 r2 t1 t2 (E: S.equal t1 t2 = false),
-  InA S.Equal t1 (F.get_trees (D2.dfs_forest g lt H o)) ->
-  InA S.Equal t2 (F.get_trees (D2.dfs_forest g lt H o)) ->
-  S.In r1 t1 ->
-  S.In v1 t1 ->
-  S.In r2 t2 ->
-  S.In v2 t2 ->
-  F.is_root (D2.dfs_forest g lt H o) r1 = true ->
-  F.is_root (D2.dfs_forest g lt H o) r2 = true ->
-  D2.f_time g lt H o r1 < D2.f_time g lt H o r2 ->
-  G.contains_edge g v1 v2 = false.
-Proof.
-  intros. destruct (G.contains_edge g v1 v2) eqn : ?.
-  - assert (G.contains_vertex g r1 = true). { eapply D2.same_vertices. 
-    apply F.is_root_5. apply H6. } 
-    assert (Hr: G.contains_vertex g r2 = true). { eapply D2.same_vertices. 
-    apply F.is_root_5. apply H7. } pose proof (D2.discovery_exists g lt0 H o r1 H9).
-    destruct H10 as [sr1]. assert (forall v, S.In v t1 -> v <> r1 -> D2.white g lt0 H o sr1 v = true). { intros.
-    assert (A:= H0).
-    apply F.get_trees_root in H0. destruct H0. assert (x = r1). { eapply F.tree_root_unique.
-    apply A. apply H0. apply H6. destruct_all. apply H13. apply H2. } subst.
-    destruct_all. clear H0. clear H13. rewrite D2.white_def. rewrite Nat.ltb_lt. rewrite H10.
-    eapply D2.descendant_iff_interval. apply H9. eapply get_tree_in_graph. apply A. apply H11.
-    apply H14. auto. apply H11. }
-    assert (forall v, S.In v t2 -> D2.white g lt0 H o sr1 v = true). { intros.
-    assert (r1 <> r2). intro. subst. omega.
-    assert (D2.d_time g lt0 H o r1 < D2.d_time g lt0 H o r2). { 
-    assert ((D2.d_time g lt0 H o r1 < D2.d_time g lt0 H o r2) \/ (D2.d_time g lt0 H o r1 = D2.d_time g lt0 H o r2)
-    \/ (D2.d_time g lt0 H o r1 > D2.d_time g lt0 H o r2)) by omega. destruct H14. apply H14. destruct H14.
-    assert (r1 = r2). eapply D2.d_times_unique. apply H9. apply Hr. apply H14. contradiction. 
-    pose proof (D2.parentheses_theorem g lt0 H o r1 r2 H9 Hr H13). destruct H15. omega. destruct H15.
-    destruct_all. assert (F.desc (D2.dfs_forest g lt0 H o) r2 r1). { eapply D2.descendant_iff_interval; try(assumption);
-    try(omega). } rewrite F.root_no_desc in H6. specialize (H6 r2). contradiction. apply F.is_root_5. apply H6.
-    omega. } destruct (O.eq_dec v r2). unfold O.eq in e. subst. rewrite D2.white_def. rewrite Nat.ltb_lt. rewrite H10.
-    apply H14. assert (F.desc (D2.dfs_forest g lt0 H o) r2 v). assert (A:= H1). apply F.get_trees_root in H1. destruct_all.
-    assert (x = r2). eapply F.tree_root_unique. apply A. all: try(eassumption). subst.
-    apply H16. auto. apply H12. rewrite D2.descendant_iff_interval in H15. rewrite D2.white_def.
-    rewrite Nat.ltb_lt. omega. apply Hr. eapply get_tree_in_graph. apply H1. apply H12. }
-    assert (F.desc (D2.dfs_forest g lt0 H o) r1 v2). { eapply D2.white_path_theorem. apply H9.
-    intros. assert (s = sr1). eapply D2.state_time_unique. omega. subst. assert (A:= H0).
-    apply F.get_trees_root in H0. destruct_all. assert ( x = r1). eapply F.tree_root_unique. apply A.
-    all: try(assumption). subst. destruct (O.eq_dec r1 v1). unfold O.eq in e. subst.
-    exists nil. rewrite D2.P.path_list_ind_rev. simplify.
-    assert (F.desc (D2.dfs_forest g lt0 H o) r1 v1). {
-    apply H15. intro. subst. apply n. reflexivity. assumption. }
-    rewrite D2.white_path_theorem in H16. specialize (H16 sr1 H13). destruct H16.
-    exists (v1 :: x). rewrite D2.P.path_list_ind_rev. rewrite D2.P.path_list_ind_rev in H16.
-    destruct_all.  simpl. simplify. subst. apply H18. apply H9. } 
-    assert (v2 <> r1). { intro. subst. rewrite F.root_no_desc in H6. specialize (H6 r1). contradiction.
-    apply F.is_root_5; assumption. } assert (S.In v2 t1). assert (A:= H0). apply F.get_trees_root in H0.
-    destruct_all. assert (x = r1). eapply F.tree_root_unique; try(apply A); try(assumption). subst.
-    apply H16. auto. apply H13. pose proof (F.get_trees_partition ((D2.dfs_forest g lt0 H o))).
-    unfold F.P.partition in H16. destruct_all.  unfold F.P.disjoint in H17. specialize (H17 
-    t1 t2 E H0 H1 v2). exfalso. apply H17; split; assumption.
-  - reflexivity.
-Qed. 
-
-(*One final lemma before the algorithm: get_trees is a partition according to G.contains_vertex*)
 Lemma get_trees_partition_graph : forall g lt H o,
   Pa.partition G.contains_vertex g (F.get_trees (D2.dfs_forest g lt H o)). 
 Proof.
@@ -690,10 +627,362 @@ Proof.
   apply D2.same_vertices. apply H2. apply H1.
 Qed.
 
-(** Kosaraju's Strongly Connected Components Algorithm **)
-Search F.desc.
+(** Further results about discovery and finish times as they relate to trees **)
+(*TODO: see about extending this/proving for the more general case *)
 
-(*TODO; maybe move this, maybe dont be so lazy also with assumptions*)
+(*Given two DFS trees t1 and t2 with roots r1 and r2, r1 is discovered before r2 iff it
+  finishes before r2*)
+Lemma root_times: forall g lt H o t1 t2 r1 r2,
+  InA S.Equal t1 (F.get_trees (D2.dfs_forest g lt H o)) ->
+  InA S.Equal t2 (F.get_trees (D2.dfs_forest g lt H o)) ->
+  S.In r1 t1 ->
+  S.In r2 t2 ->
+  F.is_root (D2.dfs_forest g lt H o) r1 = true ->
+  F.is_root (D2.dfs_forest g lt H o) r2 = true ->
+  D2.f_time g lt H o r1 < D2.f_time g lt H o r2 <-> D2.d_time g lt H o r1 < D2.d_time g lt H o r2.
+Proof.
+  intros. assert (G.contains_vertex g r1 = true). eapply get_tree_in_graph. apply H0. assumption.
+  assert (G.contains_vertex g r2 = true). eapply get_tree_in_graph. apply H1. assumption.
+  destruct (O.eq_dec r1 r2). unfold O.eq in e. subst. omega.
+  assert (r1 <> r2) by auto. clear n. pose proof (D2.parentheses_theorem g lt0 H o r1 r2 H6 H7 H8).
+  destruct H9.
+  - assert (F.desc (D2.dfs_forest g lt0 H o) r1 r2). eapply D2.descendant_iff_interval; try(assumption); try(omega).
+    eapply F.root_no_desc in H5. exfalso. apply H5. apply H10. eapply D2.same_vertices. assumption.
+  - destruct H9.
+    + assert (F.desc (D2.dfs_forest g lt0 H o) r2 r1). eapply D2.descendant_iff_interval; try(assumption); try(omega).
+      eapply F.root_no_desc in H4. exfalso. apply H4. apply H10. eapply D2.same_vertices. assumption.
+    + omega.
+Qed.
+
+(*Given 2 DFS trees t1 and t2 and roots r1 and r2, if r1 finishes before r2, then r1 finishes before r2 starts*)
+Lemma root_start_end: forall g lt H o t1 t2 r1 r2,
+  InA S.Equal t1 (F.get_trees (D2.dfs_forest g lt H o)) ->
+  InA S.Equal t2 (F.get_trees (D2.dfs_forest g lt H o)) ->
+  S.In r1 t1 ->
+  S.In r2 t2 ->
+  F.is_root (D2.dfs_forest g lt H o) r1 = true ->
+  F.is_root (D2.dfs_forest g lt H o) r2 = true ->
+  D2.f_time g lt H o r1 < D2.f_time g lt H o r2 ->
+  D2.f_time g lt H o r1 < D2.d_time g lt H o r2.
+Proof.
+  intros. assert (G.contains_vertex g r1 = true). eapply get_tree_in_graph. apply H0. assumption.
+  assert (G.contains_vertex g r2 = true). eapply get_tree_in_graph. apply H1. assumption.
+  destruct (O.eq_dec r1 r2). unfold O.eq in e. subst. omega.
+  assert (r1 <> r2) by auto. clear n. pose proof (D2.parentheses_theorem g lt0 H o r1 r2 H7 H8 H9).
+  destruct H10.
+  - assert (F.desc (D2.dfs_forest g lt0 H o) r1 r2). eapply D2.descendant_iff_interval; try(assumption); try(omega).
+    eapply F.root_no_desc in H5. exfalso. apply H5. apply H11. eapply D2.same_vertices. assumption.
+  - destruct H10.
+    + assert (F.desc (D2.dfs_forest g lt0 H o) r2 r1). eapply D2.descendant_iff_interval; try(assumption); try(omega).
+      eapply F.root_no_desc in H4. exfalso. apply H4. apply H11. eapply D2.same_vertices. assumption.
+    + omega.
+Qed.
+    
+(*Let t1 and t2 be 2 DFS trees with roots r1 and r2. Let u be in t1 and v be in t2. Then u finishes
+  before v is discovered*)
+Lemma tree_times: forall g lt H o t1 t2 u v r1 r2,
+  InA S.Equal t1 (F.get_trees (D2.dfs_forest g lt H o)) ->
+  InA S.Equal t2 (F.get_trees (D2.dfs_forest g lt H o)) ->
+  S.In r1 t1 ->
+  S.In r2 t2 ->
+  F.is_root (D2.dfs_forest g lt H o) r1 = true ->
+  F.is_root (D2.dfs_forest g lt H o) r2 = true ->
+  D2.f_time g lt H o r1 < D2.f_time g lt H o r2 ->
+  S.In u t1 ->
+  S.In v t2 ->
+  D2.f_time g lt H o u < D2.d_time g lt H o v.
+Proof.
+  intros. assert (G.contains_vertex g u = true).
+  eapply get_tree_in_graph. apply H0. apply H7.
+  assert (G.contains_vertex g v = true). eapply get_tree_in_graph. apply H1. apply H8.
+  assert (A :~S.In v t1 /\ ~S.In u t2). { split; intro;
+  pose proof (get_trees_partition_graph g lt0 H o); unfold Pa.partition in H12;
+  destruct_all; specialize (H13 t1 t2); destruct (S.equal t1 t2) eqn : ?.
+  - apply S.equal_2 in Heqb; rewrite <- Heqb in H3.  assert (r1 = r2). { eapply F.tree_root_unique.
+    apply H0. apply H4. apply H5. apply H2. apply H3. } subst. omega.
+  - assert (Pa.disjoint t1 t2). apply H13. reflexivity. assumption. assumption. unfold Pa.disjoint in H14.
+    apply (H14 v). split; assumption.
+  - apply S.equal_2 in Heqb; rewrite <- Heqb in H3.  assert (r1 = r2). { eapply F.tree_root_unique.
+    apply H0. apply H4. apply H5. apply H2. apply H3. } subst. omega.
+  - assert (Pa.disjoint t1 t2). apply H13. reflexivity. assumption. assumption. unfold Pa.disjoint in H14.
+    apply (H14 u). split; assumption. }
+  assert (u <> v). { intro. subst. destruct_all. contradiction. }
+  pose proof (D2.parentheses_theorem g lt0 H o u v H9 H10 H11). destruct H12.
+  - assert (F.desc (D2.dfs_forest g lt0 H o) u v). eapply D2.descendant_iff_interval. apply H9.
+    apply H10. omega. assert (F.desc (D2.dfs_forest g lt0 H o) r1 v). { assert (R:=H0).
+    apply F.get_trees_root in H0. destruct_all. assert (x = r1). eapply F.tree_root_unique.
+    apply R. all: try(assumption). subst. destruct (O.eq_dec u r1). unfold O.eq in e. subst. assumption.
+    eapply F.is_descendant_trans. apply (H19 u). auto. assumption. assumption. }
+    assert (S.In v t1). { assert (R:=H0).
+    apply F.get_trees_root in H0. destruct_all. assert (x = r1). eapply F.tree_root_unique.
+    apply R. assumption. assumption. assumption. assumption. subst. destruct (O.eq_dec v r1). unfold O.eq in e.
+    subst. assumption. apply H20. auto. assumption. } destruct_all; contradiction.
+  - destruct H12.
+    +  assert (F.desc (D2.dfs_forest g lt0 H o) v u). eapply D2.descendant_iff_interval. apply H10.
+    apply H9. omega. assert (F.desc (D2.dfs_forest g lt0 H o) r2 u). { assert (R:=H1).
+    apply F.get_trees_root in H1. destruct_all. assert (x = r2). eapply F.tree_root_unique.
+    apply R. all: try(assumption). subst. destruct (O.eq_dec v r2). unfold O.eq in e. subst. assumption.
+    eapply F.is_descendant_trans. apply (H19 v). auto. assumption. assumption. }
+    assert (S.In u t2). { assert (R:=H1).
+    apply F.get_trees_root in H1. destruct_all. assert (x = r2). eapply F.tree_root_unique.
+    apply R. assumption. assumption. assumption. assumption. subst. destruct (O.eq_dec u r2). unfold O.eq in e.
+    subst. assumption. apply H20. auto. assumption. } destruct_all; contradiction.
+    + destruct H12.
+      * omega.
+      * assert (R1 := H0). assert (R2 := H1). eapply F.get_trees_root in H0. eapply F.get_trees_root in H1.
+        destruct_all. assert (x0 = r1). eapply F.tree_root_unique. apply R1. all: try(assumption). subst.
+        assert (x = r2). eapply F.tree_root_unique. apply R2. all: try(assumption). subst.
+        destruct (O.eq_dec u r1). unfold O.eq in e. subst. destruct (O.eq_dec v r2). unfold O.eq in e. subst.
+        omega. assert (F.desc (D2.dfs_forest g lt0 H o) r2 v). eapply H18. auto. assumption.
+        eapply D2.descendant_iff_interval in H21. assert (D2.d_time g lt0 H o r1 < D2.d_time g lt0 H o r2).
+        eapply root_times. apply R1. apply R2. all: try(assumption). omega. eapply get_tree_in_graph.
+        apply R2. assumption. 
+        assert (F.desc (D2.dfs_forest g lt0 H o) r1 u). eapply H20. auto. assumption.
+        eapply D2.descendant_iff_interval in H21. assert (D2.d_time g lt0 H o r1 < D2.d_time g lt0 H o r2).
+        eapply root_times. apply R1. apply R2. all: try(assumption). destruct (O.eq_dec v r2). unfold O.eq in e.
+        subst. omega.  assert (F.desc (D2.dfs_forest g lt0 H o) r2 v). eapply H18. auto. assumption.
+        eapply D2.descendant_iff_interval in H23. eapply root_start_end in H6. omega. apply R1. apply R2.
+        all: try(assumption). eapply get_tree_in_graph. apply R2. assumption. 
+        eapply get_tree_in_graph. apply R1. assumption.
+Qed. 
+
+(** Finding the minimum element of a path **)
+(*Because a path has the start, end, and intermediate list, this basically boils down to a ton of cases*)
+
+Definition min_elt_path (u v : O.t) (f: O.t -> nat) l :=
+  match (min_elt_list l f) with
+  | Some x => if f u <? f x then 
+                if f u <? f v then u 
+                else v
+             else if f v <? f x then v else x
+  | None => if f u <? f v then u else v
+  end.
+
+Ltac destruct_if := 
+  match goal with
+  | [H : (if ?a <? ?b then _ else _) = _ |- _ ] => (destruct (a <? b) eqn : ?)
+  end.
+
+Lemma min_elt_path_in: forall u v l f x,
+  min_elt_path u v f l = x ->
+  x = u \/ x = v \/ In x l.
+Proof.
+  intros. unfold min_elt_path in H. destruct (min_elt_list l f) eqn : ?.
+  repeat(destruct_if; try(simplify)). subst.
+  right. right. apply min_elt_list_in_list in Heqo. assumption.
+  destruct_if; inversion H; simplify.
+Qed.
+
+Lemma min_elt_path_finds_min: forall u v l f x,
+  (forall x0 y0 : O.t, (u = x0 \/ v = x0 \/ In x0 l) -> (u = y0 \/ v = y0 \/ In y0 l) -> f x0 = f y0 -> x0 = y0) ->
+  ~In u l -> ~In v l -> u <> v ->
+  min_elt_path u v f l = x ->
+  (forall y, y = u \/ y = v \/ In y l -> y <> x -> f x < f y).
+Proof.
+  intros. unfold min_elt_path in H3. destruct (min_elt_list l f) eqn : ?.
+  repeat((destruct_if); repeat(rewrite Nat.ltb_lt in *)); subst.
+  simplify; subst; try(assumption); try(omega). destruct (O.eq_dec y t). unfold O.eq in e. subst.
+  assumption. eapply min_elt_list_finds_min in Heqo. assert (f t < f y) by apply Heqo. omega.
+  intros; apply H; try(right; right; assumption); assumption. apply H4. auto.
+  assert (f x < f u). { rewrite Nat.ltb_antisym in Heqb0. rewrite negb_false_iff in Heqb0.
+  apply Nat.leb_le in Heqb0. assert ( f x < f u \/ f x = f u) by omega. destruct H3. apply H3.
+  apply H in H3. subst. contradiction. right. left. reflexivity. left. reflexivity. }
+  clear Heqb0. simplify; subst; try(assumption); try(omega).
+  destruct (O.eq_dec t y). unfold O.eq in e. subst. omega. eapply min_elt_list_finds_min in Heqo.
+  assert (f t < f y) by apply Heqo. omega. intros; apply H; try(right; right; assumption); assumption. 
+  apply H4. auto. assert (f t < f u). { rewrite Nat.ltb_antisym in Heqb. rewrite negb_false_iff in Heqb.
+  apply Nat.leb_le in Heqb. assert (f t < f u \/ f t = f u) by omega. destruct H3.
+  apply H3. subst. eapply H in H3. subst. apply min_elt_list_in_list in Heqo. contradiction.
+  right. right. apply min_elt_list_in_list in Heqo; assumption. left. reflexivity. }
+  clear Heqb.  simplify; subst; try(assumption); try(omega). destruct (O.eq_dec y t). unfold O.eq in e.
+  subst. omega. eapply min_elt_list_finds_min in Heqo. assert (f t < f y) by apply Heqo. omega.
+  intros; apply H; try(right; right; assumption); assumption.  apply H4. auto.
+  assert ( f x < f v). { rewrite Nat.ltb_antisym in Heqb0. rewrite negb_false_iff in Heqb0.
+  apply Nat.leb_le in Heqb0. assert ( f x < f v \/ f x = f v) by omega. destruct H3. apply H3.
+  apply H in H3. subst. apply min_elt_list_in_list in Heqo. contradiction. right. right.
+  eapply min_elt_list_in_list. apply Heqo. right. left. reflexivity. } clear Heqb0.
+  assert ( f x < f u). { rewrite Nat.ltb_antisym in Heqb. rewrite negb_false_iff in Heqb.
+  apply Nat.leb_le in Heqb. assert (f x < f u \/ f x = f u) by omega. destruct H6.
+  apply H6. subst. eapply H in H6. subst. apply min_elt_list_in_list in Heqo. contradiction.
+  right. right. apply min_elt_list_in_list in Heqo; assumption. left. reflexivity. }
+  clear Heqb. simplify; subst; try(assumption); try(omega).
+  eapply min_elt_list_finds_min in Heqo. apply Heqo.  intros; apply H; try(right; right; assumption).
+  assumption. assumption. auto. destruct_if; repeat( rewrite Nat.ltb_lt in *); subst.
+  simplify; subst; try(assumption); try(omega). apply min_elt_list_none_iff_empty in Heqo. subst.
+  inversion H4. assert (f x < f u). { rewrite Nat.ltb_antisym in Heqb. rewrite negb_false_iff in Heqb.
+  apply Nat.leb_le in Heqb. assert ( f x < f u \/ f x = f u) by omega. destruct H3. apply H3.
+  apply H in H3. subst. contradiction. right. left. reflexivity. left. reflexivity. }
+  clear Heqb. simplify; subst; try(assumption); try(omega).  
+  apply min_elt_list_none_iff_empty in Heqo. subst. inversion H4.
+Qed.
+
+(*Why we cared about this: every path has a vertex along it that was discovered first*)
+Lemma path_has_first_discovered: forall g u v l lt H,
+  Pa.path_list_rev g u v l = true ->
+  NoDup l -> ~In u l -> ~In v l ->
+   u <> v ->
+  exists x, (x = u \/ x = v \/ In x l) /\ (forall y,  (y = u \/ y = v \/ In y l) ->y <> x ->
+  D2.d_time g lt H None x < D2.d_time g lt H None y).
+Proof.
+  intros.
+  remember (min_elt_path u v (D2.d_time g lt0 H None) l) as y.
+  exists y. split. symmetry in Heqy. eapply min_elt_path_in in Heqy. simplify. 
+  eapply min_elt_path_finds_min. intros.
+  pose proof (Pa.path_implies_in_graph g u v l H0).
+  eapply D2.d_times_unique. destruct H5. subst. simplify. destruct H5; subst; simplify.
+  destruct H6. subst. simplify. destruct H6; subst; simplify. apply H7. 
+  all: symmetry in Heqy; assumption.
+Qed.
+
+(*This is a key result towards proving the correctness of Kosaraju's Algorithm: There are no paths
+  from an earlier DFS tree to a later tree*)
+(*The proof turns out to be quite complicated.
+  Essentially, assume there is a path and let x be the element in the path that is first discovered.
+  If x is in t2 (the later tree), this contradicts the fact that u, the starting vertex, was in an
+  earlier tree. If x is in an earlier tree, then v (the end vertex) becomes a descendant of x by
+  the white path theorem, so v is in an earlier tree, which contradicts the fact that any two
+  DFS trees are djsoint.*)
+Lemma no_path_to_later_tree: forall g lt H t1 t2 r1 r2 u v,
+  InA S.Equal t1 (F.get_trees (D2.dfs_forest g lt H None)) ->
+  InA S.Equal t2 (F.get_trees (D2.dfs_forest g lt H None)) ->
+  S.In r1 t1 ->
+  S.In r2 t2 ->
+  F.is_root (D2.dfs_forest g lt H None) r1 = true ->
+  F.is_root (D2.dfs_forest g lt H None) r2 = true ->
+  D2.f_time g lt H None r1 < D2.f_time g lt H None r2 ->
+  S.In u t1 ->
+  S.In v t2 ->
+  ~Pa.path g u v.
+Proof.
+  intros. intro. assert (D2.f_time g lt0 H None u < D2.d_time g lt0 H None v). eapply tree_times.
+  apply H0. apply H1. apply H2. apply H3. all: try assumption.
+  assert (G.contains_vertex g v = true). eapply get_tree_in_graph. apply H1. assumption.
+  assert (G.contains_vertex g u = true). eapply get_tree_in_graph. apply H0. assumption.
+  assert (A :~S.In v t1 /\ ~S.In u t2). { split; intro;
+  pose proof (get_trees_partition_graph g lt0 H None); unfold Pa.partition in H14;
+  destruct_all; specialize (H15 t1 t2); destruct (S.equal t1 t2) eqn : ?.
+  - apply S.equal_2 in Heqb; rewrite <- Heqb in H3.  assert (r1 = r2). { eapply F.tree_root_unique.
+    apply H0. all: try assumption. }  subst. omega.
+  - assert (Pa.disjoint t1 t2). apply H15. reflexivity. assumption. assumption. unfold Pa.disjoint in H16.
+    apply (H16 v). split; assumption.
+  - apply S.equal_2 in Heqb; rewrite <- Heqb in H3.  assert (r1 = r2). { eapply F.tree_root_unique.
+    apply H0. all: try assumption. }  subst. omega.
+  - assert (Pa.disjoint t1 t2). apply H15. reflexivity. assumption. assumption. unfold Pa.disjoint in H16.
+    apply (H16 u). split; assumption. } destruct A as [N1 N2].
+  assert (N: u <> v). intro. subst. contradiction.
+  rewrite Pa.path_path_list_rev in H9. destruct H9 as [l]. eapply Pa.path_no_dups in H9.
+  destruct H9 as [ld]. destruct_all. assert (A:= H9). apply (path_has_first_discovered _ _ _ _ _ H) in A.
+  destruct A as [fst]. destruct_all. assert (R1 := H0). assert (R2 := H1). eapply F.get_trees_root in H0.
+  destruct H0 as [x]. destruct H0 as [HR1 HI1]. destruct HI1 as [HI1 HD1]. assert (x = r1). eapply F.tree_root_unique.
+  apply R1. all: try assumption. subst. eapply F.get_trees_root in H1. destruct H1 as [x]. destruct H0 as [HR2 HI2].
+  destruct HI2 as [HI2 HD2]. assert (x = r2). eapply F.tree_root_unique. apply R2. all: try assumption. subst. 
+  clear HR1. clear HR2. clear HI1. clear HI2. 
+  destruct H17. subst. 
+  - assert (F.desc (D2.dfs_forest g lt0 H None) u v). { eapply D2.white_path_theorem. apply H12. intros.
+    exists ld. rewrite D2.P.path_list_ind_rev. split. apply H9. split.
+    + intros. rewrite D2.white_def. rewrite H0. rewrite Nat.ltb_lt. apply H18. simplify. intro. subst. contradiction.
+    + rewrite D2.white_def. rewrite H0. rewrite Nat.ltb_lt. apply H18. simplify. intro. subst. contradiction. }
+   assert (F.desc (D2.dfs_forest g lt0 H None) r1 v). destruct (O.eq_dec r1 u). unfold O.eq in e. subst.
+   assumption. eapply F.is_descendant_trans. apply (HD1 u). auto. assumption. assumption.
+   rewrite <- HD1 in H1. contradiction. intro. subst. contradiction.
+  - destruct H0. 
+    + subst. specialize (H18 u). assert (D2.d_time g lt0 H None v < D2.d_time g lt0 H None u).
+      apply H18. left. reflexivity. apply N.
+      assert (D2.d_time g lt0 H None u < D2.f_time g lt0 H None u). 
+      pose proof (D2.parentheses_theorem g lt0 H None u v H12 H11 N). omega. omega.
+    + destruct (P2.In_dec fst t2).
+      * specialize (H18 u). assert (D2.d_time g lt0 H None fst < D2.d_time g lt0 H None u).
+        apply H18. left. reflexivity. intro. subst. contradiction.
+        assert (D2.f_time g lt0 H None u < D2.d_time g lt0 H None fst). eapply tree_times.
+        apply R1. apply R2. apply H2. apply H3. all: try assumption.
+        assert (D2.d_time g lt0 H None u < D2.f_time g lt0 H None u). 
+        pose proof (D2.parentheses_theorem g lt0 H None u v H12 H11 N). omega. omega.
+      * assert (G.contains_vertex g fst = true). eapply Pa.path_implies_in_graph.
+        apply H9. apply H0. pose proof (get_trees_partition_graph g lt0 H None).
+        unfold Pa.partition in H17. destruct H17. specialize (H17 _ H1). destruct H17 as [t3].
+        destruct H17 as [R3 H17]. assert (A:= R3). eapply F.get_trees_root in A. destruct A as [r3].
+        destruct H20 as [HR3 HI3]. destruct HI3 as [HI3 HD3].
+        assert (D2.f_time g lt0 H None r3 > D2.f_time g lt0 H None r2 \/ 
+                D2.f_time g lt0 H None r3 = D2.f_time g lt0 H None r2 \/
+                D2.f_time g lt0 H None r3 < D2.f_time g lt0 H None r2) by omega.
+        destruct H20.
+        -- assert (D2.f_time g lt0 H None r2 < D2.d_time g lt0 H None r3). eapply root_start_end.
+           apply R2. apply R3. all: try assumption. 
+           destruct (O.eq_dec v r2). unfold O.eq in e. subst. destruct (O.eq_dec fst r3). unfold O.eq in e.
+           subst. specialize (H18 r2). assert (D2.d_time g lt0 H None r3 < D2.d_time g lt0 H None r2).
+           apply H18. simplify. intro. subst. contradiction. 
+           assert (D2.d_time g lt0 H None r2 < D2.f_time g lt0 H None r2). assert (r2 <> u) by auto.
+           pose proof (D2.parentheses_theorem g lt0 H None r2 u H11 H12 H23). omega. omega.
+           assert (F.desc (D2.dfs_forest g lt0 H None) r3 fst). apply HD3. auto. assumption.
+           apply D2.descendant_iff_interval in H22. specialize (H18 r2).
+           assert (D2.d_time g lt0 H None fst < D2.d_time g lt0 H None r2). apply H18. simplify.
+           intro. subst. contradiction. 
+            assert (D2.d_time g lt0 H None r2 < D2.f_time g lt0 H None r2). assert (r2 <> u) by auto.
+           pose proof (D2.parentheses_theorem g lt0 H None r2 u H11 H12 H24). omega. omega.
+           eapply get_tree_in_graph. apply R3. assumption. assumption.
+           assert (F.desc (D2.dfs_forest g lt0 H None) r2 v). apply HD2. auto. assumption.
+           eapply D2.descendant_iff_interval in H22. destruct (O.eq_dec fst r3). unfold O.eq in e. subst.
+            specialize (H18 v). assert (D2.d_time g lt0 H None r3 < D2.d_time g lt0 H None v). apply H18.
+            simplify. intro. subst. contradiction. omega.
+            assert (F.desc (D2.dfs_forest g lt0 H None) r3 fst). apply HD3. auto. assumption.
+            apply D2.descendant_iff_interval in H23. specialize (H18 v).
+            assert (D2.d_time g lt0 H None fst < D2.d_time g lt0 H None v). apply H18. simplify.
+            intro. subst. contradiction.  omega. eapply get_tree_in_graph. apply R3. assumption.
+            assumption. eapply get_tree_in_graph. apply R2. assumption. assumption.
+        -- destruct H20.
+           ++ assert (r3 = r2). eapply D2.f_times_unique. eapply get_tree_in_graph. apply R3. assumption.
+              eapply get_tree_in_graph. apply R2. assumption. apply H20. subst.
+              destruct (S.equal t2 t3) eqn : ?. apply S.equal_2 in Heqb. rewrite Heqb in n. contradiction.
+              apply H19 in Heqb. unfold Pa.disjoint in Heqb. apply (Heqb r2). split; assumption.
+              assumption. assumption.
+           ++ assert (A:= H0). eapply in_split_app_fst in A. destruct A as [l1]. destruct H21 as  [l2].
+              destruct H21; subst. apply Pa.path_app in H9. destruct H9 as [HP1 HP2].
+              assert (F.desc (D2.dfs_forest g lt0 H None) fst v). eapply D2.white_path_theorem.
+              assumption. intros. exists l1. rewrite D2.P.path_list_ind_rev. split.
+              assumption. split. intros. rewrite D2.white_def. rewrite H9. rewrite Nat.ltb_lt.
+              apply H18. simplify. intro. subst. apply (H22 fst). apply H21. reflexivity.
+              rewrite D2.white_def. rewrite H9. rewrite Nat.ltb_lt. apply H18. simplify.
+              intro. subst. contradiction. destruct (O.eq_dec fst r3). unfold O.eq in e. subst.
+              rewrite <- HD3 in H9. destruct (S.equal t2 t3) eqn : ?. apply S.equal_2 in Heqb.
+              rewrite Heqb in n. contradiction. apply H19 in Heqb. unfold Pa.disjoint in Heqb.
+              apply (Heqb v). split; assumption. assumption. assumption. intro. subst. contradiction.
+              assert (F.desc (D2.dfs_forest g lt0 H None) r3 v). eapply F.is_descendant_trans. apply (HD3 fst).
+              auto. assumption. assumption. rewrite <- HD3 in H21. destruct (S.equal t2 t3) eqn : ?.
+              apply S.equal_2 in Heqb. rewrite Heqb in n. contradiction. apply H19 in Heqb.
+              unfold Pa.disjoint in Heqb. apply (Heqb v). split; assumption. assumption. assumption.
+              intro. subst. apply F.desc_neq in H21. contradiction. apply O.eq_dec.
+Qed.
+
+(*If vertex u is in DFS tree t and in scc C, then C is a subset of t*)
+Lemma scc_subset: forall t u c g lt Ho,
+  InA S.Equal t (F.get_trees (D2.dfs_forest g lt Ho None)) ->
+  S.In u t ->
+  S.In u c ->
+  scc c g ->
+  (forall y, S.In y c -> S.In y t).
+Proof.
+  intros. pose proof (get_trees_partition_graph g lt0 Ho None). pose proof (scc_partition_2 _ _ _ _ _ H2 H4 H H1 H0).
+  destruct H5. apply H5. apply H3. destruct H5 as [a]. destruct H5 as [b]. destruct H5 as [t'].
+  destruct_all. assert (P1 := H). assert (P2 := H6). apply F.get_trees_root in H. destruct H as [r1].
+  apply F.get_trees_root in H6. destruct H6 as [r2]. destruct_all.
+  assert (D2.f_time g lt0 Ho None r1 < D2.f_time g lt0 Ho None r2 \/
+          D2.f_time g lt0 Ho None r1 = D2.f_time g lt0 Ho None r2 \/
+          D2.f_time g lt0 Ho None r1 > D2.f_time g lt0 Ho None r2) by omega.
+  assert (S := H2). unfold scc in H2. destruct H2. unfold strongly_connected in H2. destruct_all.
+  assert (a <> b). { intro. subst. unfold Pa.partition in H4. destruct_all. apply H20 in H5.
+  unfold Pa.disjoint in H5. apply (H5 b). split; assumption. all: try assumption. }
+  destruct H16.
+  - assert (Pa.path g a b). apply H19. all: try assumption. exfalso. eapply no_path_to_later_tree.
+    apply P1. apply P2. apply H14. apply H12. assumption. assumption. assumption. apply H9.
+    apply H10. apply H21.
+  - destruct H16.
+    + assert (r1 = r2). eapply D2.f_times_unique. eapply get_tree_in_graph. apply P1. assumption.
+      eapply get_tree_in_graph. apply P2. assumption. apply H16. subst.
+      unfold Pa.partition in H4. destruct H4. apply H21 in H5. unfold Pa.disjoint in H5.
+      specialize (H5 r2). exfalso. apply H5. split; assumption. all: try assumption.
+    + exfalso. eapply no_path_to_later_tree. apply P2. apply P1. apply H12. apply H14.
+      assumption. assumption. omega. apply H10. apply H9. constructor. apply H11.
+Qed.
 
 Lemma desc_path: forall u v l,
   u <> v ->
@@ -705,80 +994,103 @@ Proof.
   - simplify. eapply D2.same_edges. apply H1. apply IHl. intros. eapply F.desc_neq.
     rewrite <- F.desc_list_iff_desc. exists l. apply H2. auto. apply H2.
 Qed. 
-Require Import Wellfounded.
 
-(*Let's try with induction*)
-
-
-Lemma strong_ind_trees: forall (P: S.t -> Prop)
-
-Lemma all_trees_strongly_connected: forall t1,
-  InA S.Equal t1 (F.get_trees (D2.dfs_forest gt lt (reverseF g') None)) ->
-  scc t1 gt.
+(*Every tree in the resulting DFS forest is strongly connected*)
+Lemma all_trees_strongly_connected: forall t,
+  InA S.Equal t (F.get_trees (D2.dfs_forest gt lt (reverseF g') None)) ->
+  strongly_connected t gt.
 Proof.
-  intros. assert (A:= H). apply F.get_trees_root in H. destruct_all.
-  clear H1. clear H0. remember (D1.f_time None g' x) as n. induction x using (@well_founded_induction G.vertex 
-                        (fun x y : G.vertex => D1.f_time None g' x < D1.f_time None g' y)
-                       (wf_inverse_image _ nat _ (@D1.f_time None g' )
-                          PeanoNat.Nat.lt_wf_0)).
-
-
-
-Lemma all_trees_strongly_connected: forall t1,
-  InA S.Equal t1 (F.get_trees (D2.dfs_forest gt lt (reverseF g') None)) ->
-  strongly_connected t1 gt.
-Proof.
-  intros. destruct (strongly_connected_dec t1 gt). apply s.
+  intros. destruct (strongly_connected_dec t gt). apply s.
   assert (A:= H). apply F.get_trees_root in H. destruct_all.
   pose proof (vertex_in_scc gt x). assert (G.contains_vertex gt x = true).
    unfold gt in A. unfold lt in A. eapply get_tree_in_graph in A. apply A.
   apply H0. specialize (H2 H3). destruct H2 as [C]. destruct_all.
-  
   assert (forall x0 : S.elt,
-      S.In x0 t1 ->
+      S.In x0 t ->
       x0 <> x ->
-      exists l : list G.vertex, Pa.path_list_rev gt x x0 l = true /\ (forall y : G.vertex, In y l -> S.In y t1)). {
+      exists l : list G.vertex, Pa.path_list_rev gt x x0 l = true /\ (forall y : G.vertex, In y l -> S.In y t)). {
   intros. apply H1 in H5. assert (x <> x0) by auto. rewrite <- F.desc_list_iff_desc in H5.
   destruct H5 as [l']. assert (B:= H5). eapply (desc_path _ _ _  H7) in H5. exists l'. simplify.
   destruct (O.eq_dec y x). unfold O.eq in e. subst. assumption. apply H1. auto.
   eapply F.desc_list_all_desc. apply B. apply H8. auto. }
-  assert ((forall x : S.elt, S.In x t1 -> G.contains_vertex gt x = true)). { intros.
+  assert ((forall x : S.elt, S.In x t -> G.contains_vertex gt x = true)). { intros.
   eapply get_tree_in_graph. apply A. apply H6. } 
-     pose proof (scc_vertex x t1 C gt H5 H6 n H2 H4 H0). clear H5.
+     pose proof (scc_vertex x t C gt H5 H6 n H2 H4 H0). clear H5.
   destruct H7 as [v]. destruct H5 as [C']. destruct_all. 
-  (*Now we have another SCC, either every vertex in t1 or in a different one - if in a tree before, then v is
-    descendant so in wrong tree. If it comes after, then that vertex should be in this tree. So it is entirely
-    within t1, but it has a later finish time, which contradicts transpose corollary and root largest finish time
-    so it must actually be strongly connected.
-  *)
-   pose proof (find_max_scc_exists (D1.f_time None g') gt C H2).
+  pose proof (find_max_scc_exists (D1.f_time None g') gt C H2).
    pose proof (find_max_scc_exists (D1.f_time None g') gt C' H8).
    destruct H12 as [fC]. destruct H13 as [fC'].
-   assert (forall y, S.In y C -> S.In y t1). {
-   pose proof (get_trees_partition_graph gt lt (reverseF g') None).
-   pose proof (scc_partition_1 _ _ _ _ _ H2 H14 A H4 H0). destruct H15. apply H15.
-   pose proof (scc_partition_2 _ _ _ _ _ H2 H14 A H4 H0). destruct H16. apply H16.
-   destruct_all. 
-     
+   assert (forall y, S.In y C -> S.In y t). { eapply scc_subset. apply A. apply H0. apply H4.
+   apply H2. }
+   assert (fC = x). { destruct (O.eq_dec fC x). apply e. 
+  assert (F.desc (D2.dfs_forest gt lt (reverseF g') None) x fC). apply H1. auto.
+  apply H14. eapply max_elt_set_in_set. apply H12. 
+  eapply D2.descendant_iff_interval in H15. assert (B:= H12). 
+  eapply max_elt_set_finds_max  in H12. assert (D1.f_time None g' x < D1.f_time None g' fC) by apply H12.
+  clear H16. pose proof (D2.discovery_exists gt lt (reverseF g') None x H3).
+  destruct H16 as [sx]. pose proof (root_largest_finish_time x sx H16 H fC).
+  assert (D1.f_time None g' x > D1.f_time None g' fC). apply H17. rewrite G.transpose_vertices.
+  apply H6. apply H14. eapply max_elt_set_in_set. apply B. rewrite D2.white_def. rewrite H16.
+  rewrite Nat.ltb_lt. omega. omega. intros. eapply D1.f_times_unique. rewrite G.transpose_vertices.
+  unfold scc in H2. destruct H2. unfold strongly_connected in s. apply s. apply H16.
+  rewrite G.transpose_vertices.
+  unfold scc in H2. destruct H2. unfold strongly_connected in H2. apply H2. apply H17. apply H18.
+  assumption. auto. assumption. unfold scc in H2. destruct H2. unfold strongly_connected in H2. apply H2.
+  eapply max_elt_set_in_set in H12. apply H12. } subst.
+  assert (F.desc (D2.dfs_forest gt lt (reverseF g') None) x fC'). apply H1. intro. subst.
+  eapply neq_scc_disjoint in H9. apply H9. split. apply max_elt_set_in_set in H12. apply H12.
+  apply max_elt_set_in_set in H13. apply H13. apply H2. apply H8. eapply scc_subset.
+  apply A. apply H5. apply H7. apply H8. eapply max_elt_set_in_set. apply H13. 
+  eapply D2.descendant_iff_interval in H15. assert (scc C g'). rewrite scc_transpose.
+  assumption. assert (scc C' g'). rewrite scc_transpose. assumption. pose proof (scc_finish_time_transpose
+  g' C C' x0 v H16 H17 x fC' H9 H11 H10 H7). unfold f_time_scc in H18. specialize (H18 H12 H13).
+  pose proof (D2.discovery_exists gt lt (reverseF g') None x H3). destruct H19 as [sx].
+  assert (D1.f_time None g' x > D1.f_time None g' fC'). eapply root_largest_finish_time.
+  apply H19. assumption. rewrite G.transpose_vertices. apply H6. eapply scc_subset.
+  apply A. apply H5. apply H7. assumption. apply max_elt_set_in_set in H13. assumption.
+  rewrite D2.white_def. rewrite H19. rewrite Nat.ltb_lt. omega. omega.
+  assumption.  apply H6. eapply scc_subset.
+  apply A. apply H5. apply H7. assumption. apply max_elt_set_in_set in H13. assumption.
+Qed.
 
-   assert (G.contains_vertex gt fC = true). unfold scc in H2. destruct H2. unfold strongly_connected in H2.
-    apply H2. eapply max_elt_set_in_set. apply H12. pose proof (get_trees_partition_graph gt lt (reverseF g') None).
-    unfold Pa.partition in H15. destruct_all. assert (FC:=H15). specialize (FC _ H14). destruct FC as [fCt FC].
-    destruct FC. assert (S.equal t1 fCt = true). { destruct (S.equal t1 fCt) eqn : ?. reflexivity.
-    
-    
-   assert (fC = x). destruct (O.eq_dec fC x). apply e. assert (B:= H12). apply max_elt_set_finds_max with (y:= x) in H12.
-   assert (F.desc (D2.dfs_forest gt lt (reverseF g') None) x fC). { apply H1. auto. eapply max_elt_set_in_set.
-   apply B.
-  
-  
-  apply not_strongly_connected_vertex in n. 
-  
-
-
+(*Finally, the proof that the algorithm is correct: Every tree in the DFS forest of the second pass
+  of DFS is a SCC*)
+Theorem scc_algorithm_correct: forall t,
+  InA S.Equal t (F.get_trees (D2.dfs_forest gt lt (reverseF g') None)) ->
+  scc t g'.
+Proof.
+  intros. rewrite scc_transpose. assert (A:= H). apply all_trees_strongly_connected in H.
+  destruct (scc_dec t gt). apply s. pose proof (non_scc_has_another t gt H n).
+  destruct H0 as [v]. destruct H0. assert (R:= A). apply F.get_trees_root in A. destruct A as [r1].
+  destruct_all. pose proof (get_trees_partition_graph gt lt (reverseF g') None). unfold Pa.partition in H5.
+  destruct H5. assert (G.contains_vertex gt v = true). { unfold strongly_connected in H1. apply H1.
+  apply S.add_1. reflexivity. } specialize (H5 _ H7). destruct H5 as [t2]. destruct H5.
+  assert (R2 := H5). apply F.get_trees_root in H5. destruct H5 as [r2]. destruct_all.
+  unfold strongly_connected in H1. destruct_all.
+  assert (r1 <> v). intro. subst. pose proof (get_trees_partition_graph gt lt (reverseF g') None).
+  unfold Pa.partition in H13. destruct H13. destruct (S.equal t t2) eqn : ?. apply S.equal_2 in Heqb.
+  rewrite Heqb in H0. contradiction. apply H14 in Heqb. unfold Pa.disjoint in Heqb.
+  apply (Heqb v). split; assumption. assumption. assumption.
+  assert (Pa.path gt r1 v). apply H12. apply S.add_2. assumption. apply S.add_1. reflexivity. apply H13.
+  assert (Pa.path gt v r1). apply H12. apply S.add_1. reflexivity. apply S.add_2. assumption. auto.  
+  assert (D2.f_time gt lt (reverseF g') None r1 < D2.f_time gt lt (reverseF g') None r2 \/
+          D2.f_time gt lt (reverseF g') None r1 = D2.f_time gt lt (reverseF g') None r2 \/
+          D2.f_time gt lt (reverseF g') None r1 > D2.f_time gt lt (reverseF g') None r2) by omega.
+  destruct H16.
+  - exfalso. eapply no_path_to_later_tree. apply R. apply R2. apply H3. apply H9. assumption.
+    assumption. assumption. apply H3. apply H8. apply H14.
+  - destruct H16.
+    + assert (r1 = r2). eapply D2.f_times_unique. eapply get_tree_in_graph. apply R.
+      assumption. eapply get_tree_in_graph. apply R2. assumption. apply H16. subst.
+      pose proof (get_trees_partition_graph gt lt (reverseF g') None).
+      unfold Pa.partition in H17. destruct H17. destruct (S.equal t t2) eqn : ?. apply S.equal_2 in Heqb.
+      rewrite Heqb in H0. contradiction. apply H18 in Heqb. unfold Pa.disjoint in Heqb.
+      exfalso. apply (Heqb r2). split; assumption. all: try assumption.
+    + exfalso. eapply no_path_to_later_tree. apply R2. apply R. apply H9. apply H3. assumption.
+      assumption. assumption. apply H8. apply H3. apply H15.
+Qed.
 
 End SecondPass.
-
 
 End SCCAlg.
 
